fill in admitted lemmas about prediction results coming from the grammar

coq/Prediction.v
@@ -115,12 +115,12 @@ Lemma subparser_lt_after_push :
     -> sp' = Sp (NtSet.remove y av) pred (callee, caller :: locs)
     -> caller = Loc x pre (NT y :: suf')
     -> callee = Loc y [] rhs
-    ->  NtSet.mem y av = true
+    ->  NtSet.In y av
     -> In rhs (rhssForNt g y)
     -> lex_nat_pair (meas g sp') (meas g sp).
 Proof.
   intros g sp sp' av pred cr ce locs x y pre suf' rhs
-         Hsp Hsp' Hcr Hce Hmem Hin; subst.
+         Hsp Hsp' Hcr Hce Hin Hin'; subst.
   unfold meas.
   apply pair_fst_lt.
   eapply stackScore_lt_after_push; simpl; eauto.
@@ -131,18 +131,29 @@ Lemma acc_after_push :
     Acc lex_nat_pair (meas g sp)
     -> sp  = Sp av pred (loc, locs)
     -> loc = Loc x pre (NT y :: suf_tl)
-    -> NtSet.mem y av = true
+    -> NtSet.In y av
     -> In sp' (map (fun rhs => Sp (NtSet.remove y av)
                                   pred
                                   (Loc y [] rhs, loc :: locs))
                    (rhssForNt g y))
     -> Acc lex_nat_pair (meas g sp').
 Proof.
-  intros g sp sp' av pred pre suf_tl loc locs x y Ha Hs Hl Hm Hin; subst.
+  intros g sp sp' av pred pre suf_tl loc locs x y Ha Hs Hl Hin Hin'; subst.
   eapply Acc_inv; eauto.
-  apply in_map_iff in Hin.
-  destruct Hin as [rhs [Heq Hin]]; subst.
+  apply in_map_iff in Hin'.
+  destruct Hin' as [rhs [Heq Hin']]; subst.
   eapply subparser_lt_after_push; eauto.
+Defined.
+
+Definition mem_dec (x : nonterminal) (s : NtSet.t) :
+  {~NtSet.In x s} + {NtSet.In x s}.
+  destruct (NtSet.mem x s) eqn:Hm.
+  - right.
+    apply NtSet.mem_spec; auto.
+  - left.
+    unfold not; intros H.
+    apply NtSet.mem_spec in H.
+    congruence.
 Defined.
 
 (* subparser closure *)
@@ -168,19 +179,17 @@ Fixpoint spc (g : grammar) (sp : subparser)
       | Loc _ _ (T _ :: _)       => fun _ => [inr sp]
       | Loc x pre (NT y :: suf') =>
         fun Hl =>
-          match NtSet.mem y av as b return NtSet.mem y av = b -> _ with
-          | true =>
-            fun Hm =>
-              let sps' :=
-                  map (fun rhs =>
-                         Sp (NtSet.remove y av) pred (Loc y [] rhs, loc :: locs))
-                      (rhssForNt g y)
-              in  dflat_map sps'
-                            (fun sp' Hi =>
-                               spc g sp' (acc_after_push _ _ a Hs Hl Hm Hi))
-                            
-          | false => fun _ => [inl clRecErr]
-          end eq_refl
+          match mem_dec y av with
+          | left _   => [inl clRecErr]
+          | right Hm =>
+            let sps' :=
+                map (fun rhs =>
+                       Sp (NtSet.remove y av) pred (Loc y [] rhs, loc :: locs))
+                    (rhssForNt g y)
+            in  dflat_map sps'
+                          (fun sp' Hi =>
+                             spc g sp' (acc_after_push _ _ a Hs Hl Hm Hi))
+          end
       end eq_refl
   end eq_refl.
 
@@ -263,7 +272,7 @@ Proof.
   eapply Forall_forall in Hf; eauto.
 Defined.
 
-Lemma filter_eq_cons_in :
+Lemma filter_cons_in :
   forall (A : Type) (f : A -> bool) (l : list A) (hd : A) (tl : list A),
     filter f l = hd :: tl
     -> In hd l.
@@ -285,7 +294,21 @@ Proof.
   dm; tc.
   inv Hh.
   eexists; split; eauto.
-  eapply filter_eq_cons_in; eauto.
+  eapply filter_cons_in; eauto.
+Defined.
+
+Lemma handleFinalSubparsers_ambig_from_subparsers :
+  forall sps gamma,
+    handleFinalSubparsers sps = PredAmbig gamma
+    -> exists sp, In sp sps /\ sp.(prediction) = gamma.
+Proof.
+  intros sps gamma Hh.
+  unfold handleFinalSubparsers in Hh.
+  dmeq Hf; tc.
+  dm; tc.
+  inv Hh.
+  eexists; split; eauto.
+  eapply filter_cons_in; eauto.
 Defined.
 
 Lemma move_unfold :
@@ -298,6 +321,54 @@ Proof.
   auto. 
 Defined.
 
+Lemma in_sumOfListSum_result_in_input :
+  forall A B (es : list (sum A B)) (b : B) (bs : list B),
+    sumOfListSum es = inr bs
+    -> In b bs
+    -> In (inr b) es.
+Proof.
+  intros A B es b.
+  induction es as [| e es' IH]; intros bs Hs Hi.
+  - simpl in *. inv Hs. inv Hi.
+  - simpl in Hs.
+    destruct e as [a | b']; tc.
+    destruct (sumOfListSum es') eqn:Htl; tc.
+    inv Hs.
+    inv Hi.
+    + apply in_eq.
+    + apply in_cons; eauto.
+Defined.
+
+Lemma in_extractSomes_result_in_input :
+  forall A (a : A) (os : list (option A)),
+    In a (extractSomes os)
+    -> In (Some a) os.
+Proof.
+  intros A a os Hi; induction os as [| o os' IH]; simpl in Hi.
+  - inv Hi.
+  - destruct o as [a' |].
+    + inv Hi.
+      * apply in_eq.
+      * apply in_cons; auto.
+    + apply in_cons; auto.
+Defined.
+
+Lemma moveSp_preserves_prediction :
+  forall t sp sp',
+    moveSp t sp = Some (inr sp')
+    -> sp'.(prediction) = sp.(prediction).
+Proof.
+  intros t sp sp' Hm.
+  unfold moveSp in Hm.
+  destruct sp as [av pred (loc, locs)].
+  destruct loc as [x pre suf].
+  destruct suf as [| [a | x'] suf_tl]; tc.
+  - destruct locs; tc.
+  - destruct t as (a', _).
+    destruct (t_eq_dec a' a); subst; tc.
+    inv Hm; auto.
+Defined.
+
 Lemma move_preserves_prediction :
   forall t sp' sps sps',
     move t sps = inr sps'
@@ -305,23 +376,151 @@ Lemma move_preserves_prediction :
     -> exists sp, In sp sps /\ sp'.(prediction) = sp.(prediction).
 Proof.
   intros s sp' sps sps' Hm Hin.
-  rewrite move_unfold in Hm.
-  simpl in Hm.
-  induction sps as [| sp sps IH]; simpl in *.
-  - inv Hm. inv Hin.
-  - destruct (moveSp s sp) eqn:Hmsp.
-    + simpl in *.
   unfold move in Hm.
-  induction 
-  unfold sumOfListSum in Hm.
-Admitted.
+  eapply in_sumOfListSum_result_in_input in Hm; eauto.
+  apply in_extractSomes_result_in_input in Hm.
+  eapply in_map_iff in Hm.
+  destruct Hm as [sp [Hmsp Hin']].
+  eexists; split; eauto.
+  eapply moveSp_preserves_prediction; eauto.
+Defined.
 
+Lemma spc_unfold_return :
+  forall g sp a es av pred stk loc locs x pre caller locs_tl x_cr pre_cr suf_cr y suf_tl_cr,
+    spc g sp a = es
+    -> sp = Sp av pred stk
+    -> stk = (loc, locs)
+    -> loc = Loc x pre []
+    -> locs = caller :: locs_tl
+    -> caller = Loc x_cr pre_cr suf_cr
+    -> suf_cr = NT y :: suf_tl_cr
+    -> exists a',
+        spc g
+            (Sp (NtSet.add y av)
+                pred
+                (Loc x_cr (pre_cr ++ [NT y]) suf_tl_cr, locs_tl))
+            a' = es.
+Proof.
+  intros.
+  subst.
+  destruct a.
+  simpl.
+  eexists; eauto.
+Defined.
+
+Lemma in_dflat_map :
+  forall (A B : Type) (l : list A) (f : forall x, In x l -> list B) (y : B) (ys : list B),
+    dflat_map l f = ys
+    -> In y ys
+    -> (exists x Hin, In x l /\ In y (f x Hin)).
+Proof.
+  intros A B l f y ys Heq Hin; subst.
+  induction l as [| x l' IH].
+  + inv Hin.
+  + simpl in Hin.
+    apply in_app_or in Hin; destruct Hin as [Hl | Hr].
+    * exists x; eexists; split; eauto.
+      apply in_eq.
+    * apply IH in Hr.
+      destruct Hr as [x' [Hin [Hin' Hin'']]].
+      exists x'; eexists; split; eauto.
+      -- apply in_cons; auto.
+      -- apply Hin''.
+Defined.
+
+(* CLEAN THIS UP! *)
+Lemma sp_closure_preserves_prediction :
+  forall g sp Ha sp' es,
+    spc g sp Ha = es
+    -> In (inr sp') es
+    -> sp'.(prediction) = sp.(prediction).
+Proof.
+  intros g sp.
+  remember (stackScore (stack sp) (S (maxRhsLength g)) (NtSet.cardinal (avail sp))) as score.
+  generalize dependent sp.
+  induction score as [score IHscore] using lt_wf_ind.
+  intros sp.
+  remember (stackHeight (stack sp)) as height.
+  generalize dependent sp.
+  induction height as [height IHheight] using lt_wf_ind.
+  intros sp Hheight Hscore Ha sp' es Hf Hi.
+  destruct Ha as [Ha].
+  destruct sp as [av pred stk] eqn:Hsp.
+  destruct stk as (loc, locs) eqn:Hstk.
+  destruct loc as [x pre suf] eqn:Hloc.
+  destruct suf as [| [a | y] suf_tl] eqn:Hsuf.
+  - (* return case *)
+    destruct locs as [| caller locs_tl] eqn:Hlocs.
+    + (* return to final configuration *)
+      simpl in Hf; subst.
+      apply in_singleton_eq in Hi; inv Hi; auto.
+    + (* return to caller frame *)
+      destruct caller as [x_cr pre_cr suf_cr] eqn:Hcr.
+      destruct suf_cr as [| [a | x'] suf_tl_cr] eqn:Hsufcr.
+      * simpl in Hf; subst.
+        apply in_singleton_eq in Hi; tc.
+      * simpl in Hf; subst.
+        apply in_singleton_eq in Hi; tc.
+      * (*eapply spc_unfold_return in Hf; eauto.
+        destruct Hf as [a' Hf]. *)
+        pose proof stackScore_le_after_return as Hss.
+        specialize Hss with
+            (callee := Loc x pre [])
+            (caller := Loc x_cr pre_cr (NT x' :: suf_tl_cr))
+            (caller' := Loc x_cr (pre_cr ++ [NT x']) suf_tl_cr)
+            (x := x')
+            (x' := x')
+            (suf' := suf_tl_cr)
+            (av := av)
+            (locs := locs_tl)
+            (b := S (maxRhsLength g)).
+        eapply le_lt_or_eq in Hss; auto.
+        destruct Hss as [Hlt | Heq].
+        -- eapply IHscore with
+               (sp := Sp (NtSet.add x' av)
+                         pred
+                         (Loc x_cr (pre_cr ++ [NT x']) suf_tl_cr,
+                          locs_tl)); subst; eauto.
+        -- eapply IHheight with
+               (sp := Sp (NtSet.add x' av)
+                         pred
+                         (Loc x_cr (pre_cr ++ [NT x']) suf_tl_cr,
+                          locs_tl)); subst; eauto.
+           simpl; auto.
+  - (* next symbol is a terminal *)
+    simpl in Hf; subst.
+    apply in_singleton_eq in Hi; inv Hi; auto.
+  - (* next symbol is a nonterminal *)
+    simpl in Hf.
+    destruct (mem_dec y av).
+    + subst; apply in_singleton_eq in Hi; inv Hi.
+    + eapply in_dflat_map in Hf; eauto.
+      destruct Hf as [sp_mid [Hin [Hin' Hf]]].
+      eapply in_map_iff in Hin'.
+      destruct Hin' as [rhs [Heq Hin']].
+      assert (Hlt : stackScore (stack sp_mid) (S (maxRhsLength g)) (NtSet.cardinal (avail sp_mid)) < score).
+      { subst.
+        eapply stackScore_lt_after_push; simpl; eauto. }
+      subst.
+      eapply IHscore in Hlt; simpl in *; eauto.
+      simpl in *; auto.
+      simpl in *; auto.
+Defined.
+  
 Lemma closure_preserves_prediction :
   forall g sp' sps sps',
     closure g sps = inr sps'
     -> In sp' sps'
     -> exists sp, In sp sps /\ sp'.(prediction) = sp.(prediction).
-Admitted.
+Proof.
+  intros g sp' sps sps' Hc Hi'.
+  unfold closure in Hc.
+  eapply in_sumOfListSum_result_in_input in Hc; eauto.
+  apply in_flat_map in Hc.
+  destruct Hc as [sp [Hi Hspc]].
+  eexists; split; eauto.
+  eapply sp_closure_preserves_prediction; eauto.
+Defined.
 
 Lemma llPredict'_success_result_in_original_subparsers :
   forall g ts gamma sps,
@@ -347,13 +546,42 @@ Proof.
       destruct Hm as [sp [Hin Heq]]; eauto.
 Defined.
 
-Lemma startState_sp_prediction_in_rhssForNt :
-  forall g x stk sp sps,
-    startState g x stk = inr sps
-    -> In sp sps
-    -> In sp.(prediction) (rhssForNt g x).
+Lemma llPredict'_ambig_result_in_original_subparsers :
+  forall g ts gamma sps,
+    llPredict' g ts sps = PredAmbig gamma
+    -> exists sp, In sp sps /\ (prediction sp) = gamma.
 Proof.
-Admitted.
+  intros g ts gamma.
+  induction ts as [| t ts_tl IH]; intros sps Hl; simpl in Hl.
+  - eapply handleFinalSubparsers_ambig_from_subparsers; eauto.
+  - destruct sps as [| sp_hd sps_tl] eqn:Hs; tc.
+    destruct (allPredictionsEqual sp_hd sps_tl) eqn:Ha; tc.
+    rewrite <- Hs in *; clear Hs. 
+    destruct (move t _) as [msg | sps'] eqn:Hm; tc.
+    destruct (closure g sps') as [msg | sps''] eqn:Hc; tc. 
+    apply IH in Hl; clear IH.
+    destruct Hl as [sp'' [Hin'' Heq]]; subst.
+    eapply closure_preserves_prediction in Hc; eauto.
+    destruct Hc as [sp' [Hin' Heq]]; rewrite Heq; clear Heq.
+    eapply move_preserves_prediction in Hm; eauto.
+    destruct Hm as [sp [Hin Heq]]; eauto.
+Defined.
+
+Lemma startState_sp_prediction_in_rhssForNt :
+  forall g x stk sp' sps',
+    startState g x stk = inr sps'
+    -> In sp' sps'
+    -> In sp'.(prediction) (rhssForNt g x).
+Proof.
+  intros g x stk sp' sps' Hf Hi.
+  unfold startState in Hf.
+  destruct stk as (loc, locs).
+  eapply closure_preserves_prediction in Hf; eauto.
+  destruct Hf as [sp [Hin Heq]]; subst.
+  apply in_map_iff in Hin.
+  destruct Hin as [gamma [Hin Heq']]; subst.
+  rewrite Heq; auto.
+Defined.  
 
 Lemma PredSucc_result_in_rhssForNt :
   forall g x stk ts gamma,
@@ -372,6 +600,12 @@ Lemma PredAmbig_result_in_rhssForNt :
   forall g x stk ts gamma,
     llPredict g x stk ts = PredAmbig gamma
     -> In gamma (rhssForNt g x).
-Admitted.
-
+Proof.
+  intros g x stk ts gamma Hf.
+  unfold llPredict in Hf.
+  dmeq Hss; tc.
+  apply llPredict'_ambig_result_in_original_subparsers in Hf.
+  destruct Hf as [sp [Hin Heq]]; subst.
+  eapply startState_sp_prediction_in_rhssForNt; eauto.
+Defined.
  
